checkpoint WiP on getting SHA to verify with new decls
Most of the changes here are to work with opaque definitions for
registers, mem and global state validity, which are intended to
decouple memory/global validity from the current state (i.e. once
I have a valid address, it's valid in every state). The problem
with this is a Dafny opaque bug (Dafny issue #63), so there are a
couple of places where we need to reveal the definitions that we
shouldn't have to. There's a lot of noise in this commit, but
most of it is purely mechanical changes from direct map indexing
for mem/globals to use indirect accessors.

Current verification status:
timeouts in sp__refined__Body__00__15, sp__refined__Body__16__XX

errors in sp__abstract__sha256__one__block,
sp__refined__sha256__loop (loop invariants) and
sp__abstract__sha256__block__data__order (register preservation)

I expect most of the errors are due to the opaque bug and hope
that rolling forward to a new Dafny will help.

verified/ARMspartan.dfy
@@ -50,6 +50,9 @@ predicate sp_require(b0:codes, c1:code, s0:sp_state, sN:sp_state)
     sp_cHeadIs(b0, c1)
  && sp_eval(Block(b0), s0, sN)
  && ValidState(s0)
+ // XXX: workaround dafny opaque bugs! these are needed in sp_refined lemmas
+ && forall regs :: ValidRegState(regs) ==> (forall r:ARMReg :: r in regs)
+ && forall mem :: ValidAddrMemStateOpaque(mem) ==> ValidAddrMemState(mem)
 }
 
 predicate sp_ensure(b0:codes, b1:codes, s0:sp_state, s1:sp_state, sN:sp_state)
@@ -96,11 +99,13 @@ function sp_get_reg(r:ARMReg, s:state):word
 }
 
 function sp_get_mem(s:state):memmap
-    ensures ValidMemState(s.m) ==> ValidAddrMemStateOpaque(sp_get_mem(s))
+    requires ValidState(s)
+    ensures ValidAddrMemStateOpaque(sp_get_mem(s))
 { reveal_ValidMemState(); reveal_ValidAddrMemStateOpaque(); s.m.addresses }
 
 function sp_get_globals(s:state):globalsmap
-    ensures ValidMemState(s.m) ==> ValidGlobalStateOpaque(sp_get_globals(s))
+    requires ValidState(s)
+    ensures ValidGlobalStateOpaque(sp_get_globals(s))
 { reveal_ValidMemState(); reveal_ValidGlobalStateOpaque(); s.m.globals }
 
 function sp_get_osp(s:state):word 
@@ -118,13 +123,17 @@ function sp_get_olr(s:state):word
 
 function sp_update_ok(sM:state, sK:state):state { sK.(ok := sM.ok, steps := sM.steps) }
 function sp_update_reg(r:ARMReg, sM:state, sK:state):state 
-    requires ValidRegState(sM.regs)
+    requires ValidRegState(sK.regs) && ValidRegState(sM.regs)
+    ensures ValidRegState(sp_update_reg(r, sM, sK).regs)
 {
     reveal_ValidRegState();
     sK.(regs := sK.regs[r := sM.regs[r]])
 }
 function sp_update_mem(sM:state, sK:state):state
+    requires ValidAddrMemStateOpaque(sM.m.addresses)
+    ensures ValidAddrMemStateOpaque(sp_update_mem(sM, sK).m.addresses)
 {
+    reveal_ValidAddrMemStateOpaque();
     sK.(m := sK.m.(addresses := sM.m.addresses))
 }
 function sp_update_globals(sM:state, sK:state):state
@@ -132,21 +141,21 @@ function sp_update_globals(sM:state, sK:state):state
     sK.(m := sK.m.(globals := sM.m.globals))
 }
 function sp_update_osp(sM:state, sK:state):state 
-    requires ValidRegState(sM.regs)
+    requires ValidRegState(sK.regs) && ValidRegState(sM.regs)
+    ensures ValidRegState(sp_update_osp(sM, sK).regs)
 { 
-    reveal_ValidRegState();
     sp_update_reg(SP(mode_of_state(sM)), sM, sK)
 }
 function sp_update_olr(sM:state, sK:state):state 
-    requires ValidRegState(sM.regs)
+    requires ValidRegState(sK.regs) && ValidRegState(sM.regs)
+    ensures ValidRegState(sp_update_olr(sM, sK).regs)
 { 
-    reveal_ValidRegState();
     sp_update_reg(LR(mode_of_state(sM)), sM, sK)
 }
 
 function sp_update(o:operand, sM:state, sK:state):state
     requires ValidRegOperand(o)
-    requires ValidRegState(sM.regs)
+    requires ValidRegState(sK.regs) && ValidRegState(sM.regs)
 {
     match o
         case OReg(r) => sp_update_reg(o.r, sM, sK)
