verified/sha/sha256-refined-invariants.i.dfy
@@ -5,6 +5,15 @@ include "../sha/sha256.i.dfy"
 include "../sha/bit-vector-lemmas.i.dfy"
 include "../ARMdecls-refined.gen.dfy"
 
+predicate SaneShaGlobal(gm: globalsmap)
+{
+ ValidGlobalStateOpaque(gm)
+ && ValidGlobal(K_SHA256s())
+ && SizeOfGlobal(K_SHA256s()) == 4*64
+ && isUInt32(AddressOfGlobal(K_SHA256s()) + 4*64) // We won't wrap around while accessing K_SHA256s
+ && forall j :: 0 <= j < 64 ==> GlobalContents(gm, K_SHA256s(), AddressOfGlobal(K_SHA256s()) + j*4) == K_SHA256(j)
+}
+
 predicate BlockInvariant(
             trace:SHA256Trace, input:seq<word>, globals:globalsmap,
             old_M_len:nat, old_mem:memmap, mem:memmap, sp:word, lr:word, r1:word, r12:word,
@@ -12,25 +21,26 @@ predicate BlockInvariant(
             input_ptr:word, ctx_ptr:word,             
             num_blocks:nat, block:nat)            
 {
+    ValidAddrMemStateOpaque(old_mem)
+ && ValidAddrMemStateOpaque(mem)
  // Stack is accessible
-    ValidAddrs(mem, sp, 19)
+ && ValidAddrs(sp, 19)
 
  // Pointer into our in-memory H[8] is valid
- && ctx_ptr == mem[sp + 16 * 4]
+ && ctx_ptr == AddrMemContents(mem, sp + 16 * 4)
  && (ctx_ptr + 32 < sp || ctx_ptr > sp + 19 * 4)
- && ValidAddrs(mem, ctx_ptr, 8)
+ && ValidAddrs(ctx_ptr, 8)
 
  // Input properties
  && block <= num_blocks
  && SeqLength(input) == num_blocks*16
  && r1 == input_ptr + block * 16 * 4
- && input_ptr + num_blocks * 16 * 4 == mem[sp + 18*4] == r12
+ && input_ptr + num_blocks * 16 * 4 == AddrMemContents(mem, sp + 18*4) == r12
  && input_ptr + num_blocks * 16 * 4 < 0x1_0000_0000
  && (input_ptr + num_blocks * 16 * 4 < sp || sp + 19 * 4 <= input_ptr)  // Doesn't alias sp
  && (input_ptr + num_blocks * 16 * 4 < ctx_ptr || ctx_ptr + 32 <= input_ptr)  // Doesn't alias input_ptr
- && ValidAddrs(mem, input_ptr, num_blocks * 16)
- && (forall j {:trigger input_ptr + j * 4 in mem} ::
-            0 <= j < num_blocks * 16 ==> mem[input_ptr + j * 4] == input[j])
+ && ValidAddrs(input_ptr, num_blocks * 16)
+ && (forall j {:trigger ValidMem(input_ptr + j * 4)} :: 0 <= j < num_blocks * 16 ==> AddrMemContents(mem, input_ptr + j * 4) == input[j])
 
  // Trace properties
  && IsCompleteSHA256Trace(trace)
@@ -40,25 +50,22 @@ predicate BlockInvariant(
              ==> trace.M[old_M_len + i] == bswap32_seq(input[i*16..(i+1)*16])) 
 
  // Globals properties
+ && SaneShaGlobal(globals)
  && ValidGlobalAddr(K_SHA256s(), lr) 
- && K_SHA256s() in globals
- && AddressOfGlobal(K_SHA256s()) + 256 < 0x1_0000_0000 
  && lr == AddressOfGlobal(K_SHA256s()) 
- && SeqLength(globals[K_SHA256s()]) == 256
- && (forall j :: 0 <= j < 64 ==> globals[K_SHA256s()][j] == K_SHA256(j))
 
  // Hs match memory and our registers
- && last(trace.H)[0] == mem[ctx_ptr + 0 * 4] == a 
- && last(trace.H)[1] == mem[ctx_ptr + 1 * 4] == b 
- && last(trace.H)[2] == mem[ctx_ptr + 2 * 4] == c 
- && last(trace.H)[3] == mem[ctx_ptr + 3 * 4] == d 
- && last(trace.H)[4] == mem[ctx_ptr + 4 * 4] == e 
- && last(trace.H)[5] == mem[ctx_ptr + 5 * 4] == f 
- && last(trace.H)[6] == mem[ctx_ptr + 6 * 4] == g 
- && last(trace.H)[7] == mem[ctx_ptr + 7 * 4] == h 
+ && last(trace.H)[0] == AddrMemContents(mem, ctx_ptr + 0 * 4) == a 
+ && last(trace.H)[1] == AddrMemContents(mem, ctx_ptr + 1 * 4) == b 
+ && last(trace.H)[2] == AddrMemContents(mem, ctx_ptr + 2 * 4) == c 
+ && last(trace.H)[3] == AddrMemContents(mem, ctx_ptr + 3 * 4) == d 
+ && last(trace.H)[4] == AddrMemContents(mem, ctx_ptr + 4 * 4) == e 
+ && last(trace.H)[5] == AddrMemContents(mem, ctx_ptr + 5 * 4) == f 
+ && last(trace.H)[6] == AddrMemContents(mem, ctx_ptr + 6 * 4) == g 
+ && last(trace.H)[7] == AddrMemContents(mem, ctx_ptr + 7 * 4) == h 
 
  // Memory framing:  We only touch the stack and 8 bytes pointed to by ctx_ptr
- && (forall addr:word :: addr in old_mem && (addr < sp || addr >= sp + 19 * 4) 
+ && (forall addr:word :: ValidMem(addr) && (addr < sp || addr >= sp + 19 * 4) 
                                          && (addr < ctx_ptr || addr >= ctx_ptr + 8 * 4) 
-                     ==> addr in mem && old_mem[addr] == mem[addr])
+                     ==> AddrMemContents(old_mem, addr) == AddrMemContents(mem, addr))
 }
