verified/sha/sha256.i.dfy
@@ -551,7 +551,9 @@ function {:opaque} bswap32_seq(input:seq<word>) : seq<word>
     else [bswap32(input[0])] + bswap32_seq(input[1..])
 }
 
-predicate ValidAddrs(mem:memmap, base:int, num_words:int)
+predicate ValidAddrs(base:int, num_words:int)
 {
-    ValidAddrMemState(mem) && ValidMem(base) && ValidMemRange(base, base + num_words * 4)
+    ValidMem(base)
+    && forall a:int {:trigger ValidMem(a)} :: base <= a < base + num_words * 4
+        ==> ValidMem(a)
 }
